Update OracleCode.lean

Project/OracleCode.lean
@@ -8,28 +8,28 @@ public import Mathlib.Computability.TuringDegree
 
 This file is a "relativized" version of `Mathlib/Computability/PartrecCode.lean`.
 
-It defines `OCode`, an inductive datatype describing codes for partial recursive functions on ℕ with an oracle. It defines an encoding for these codes, and proves that the constructors are primitive recursive with respect to the encoding.
+It defines `Code`, an inductive datatype describing codes for partial recursive functions on ℕ with an oracle. It defines an encoding for these codes, and proves that the constructors are primitive recursive with respect to the encoding.
 
-Note that although `RecursiveIn` takes a set of oracles, `OCode` allows just a single oracle. Another option would have been to allow a family of oracles indexed by a `Primcodable` type (i.e., we would define a structure `OCode (α : Type*) [Primcodable α]`). But (1) such a family can be computably encoded as a single oracle anyway, and (2) the need to consider indexed families of oracles seems rare enough that it was not worth the extra complication.
+Note that although `RecursiveIn` takes a set of oracles, `Code` allows just a single oracle. Another option would have been to allow a family of oracles indexed by a `Primcodable` type (i.e., we would define a structure `Code (α : Type*) [Primcodable α]`). But (1) such a family can be computably encoded as a single oracle anyway, and (2) the need to consider indexed families of oracles seems rare enough that it was not worth the extra complication.
 
-It also defines the evaluation of an `OCode` as a partial function, and proves that a function `f` is Turing reducible to `g` if and only if it is the evaluation of some `OCode` using `g` as an oracle.
+It also defines the evaluation of an `Code` as a partial function, and proves that a function `f` is Turing reducible to `g` if and only if it is the evaluation of some `Code` using `g` as an oracle.
 
 ## Main Definitions
 
-* `RecursiveIn.OCode`: Inductive datatype for partial recursive functions with an oracle.
-* `RecursiveIn.OCode.encodeOCode`: A (computable) encoding of an `OCode` as a natural number.
-* `RecursiveIn.OCode.ofNatOCode`: The inverse of this encoding.
-* `RecursiveIn.OCode.eval`: The interpretation of an `OCode` as a partial function.
+* `RecursiveIn.Code`: Inductive datatype for partial recursive functions with an oracle.
+* `RecursiveIn.Code.encodeCode`: A (computable) encoding of an `Code` as a natural number.
+* `RecursiveIn.Code.ofNatCode`: The inverse of this encoding.
+* `RecursiveIn.Code.eval`: The interpretation of an `Code` as a partial function.
 
 ## Main Results
 
-* `RecursiveIn.OCode.primrec_recOn`: Recursion on `RecursiveIn.OCode` is primitive recursive.
-* `RecursiveIn.OCode.computable_recOn`: Recursion on `RecursiveIn.OCode` is computable.
-* `RecursiveIn.OCode.smn`: The $S_n^m$ theorem.
-* `RecursiveIn.OCode.exists_code`: Being Turing reducible to `g` is equivalent to being the eval of an `OCode` with oracle `g`.
-* `RecursiveIn.OCode.primrec_evaln`: `evaln` is primitive recursive.
-* `RecursiveIn.OCode.fixed_point`: Roger's fixed point theorem.
-* `RecursiveIn.OCode.fixed_point₂`: Kleene's second recursion theorem.
+* `RecursiveIn.Code.primrec_recOn`: Recursion on `RecursiveIn.Code` is primitive recursive.
+* `RecursiveIn.Code.computable_recOn`: Recursion on `RecursiveIn.Code` is computable.
+* `RecursiveIn.Code.smn`: The $S_n^m$ theorem.
+* `RecursiveIn.Code.exists_code`: Being Turing reducible to `g` is equivalent to being the eval of an `Code` with oracle `g`.
+* `RecursiveIn.Code.primrec_evaln`: `evaln` is primitive recursive.
+* `RecursiveIn.Code.fixed_point`: Roger's fixed point theorem.
+* `RecursiveIn.Code.fixed_point₂`: Kleene's second recursion theorem.
 -/
 
 @[expose] public section
@@ -64,77 +64,77 @@ theorem rfind' {O f} (hf : RecursiveIn O f) :
   --   simpa
 
 /-- Code for partial recursive functions from ℕ to ℕ with an oracle.
-See `RecursiveIn.OCode.eval` for the interpretation of these constructors.
+See `RecursiveIn.Code.eval` for the interpretation of these constructors.
 -/
-inductive OCode : Type
-  | zero : OCode
-  | succ : OCode
-  | left : OCode
-  | right : OCode
-  | oracle : OCode
-  | pair : OCode → OCode → OCode
-  | comp : OCode → OCode → OCode
-  | prec : OCode → OCode → OCode
-  | rfind' : OCode → OCode
+inductive Code : Type
+  | zero : Code
+  | succ : Code
+  | left : Code
+  | right : Code
+  | oracle : Code
+  | pair : Code → Code → Code
+  | comp : Code → Code → Code
+  | prec : Code → Code → Code
+  | rfind' : Code → Code
 
-compile_inductive% OCode
+compile_inductive% Code
 
 end RecursiveIn
 
-namespace RecursiveIn.OCode
+namespace RecursiveIn.Code
 
 open Nat Nat.Partrec
 
-/-- A `Nat.Partrec.Code` can be converted to a `RecursiveIn.OCode`. -/
-def ofCode : Code → OCode
+/-- A `Nat.Partrec.Code` can be converted to a `RecursiveIn.Code`. -/
+def ofPartrecCode : Nat.Partrec.Code → Code
   | .zero => zero
   | .succ => succ
   | .left => left
   | .right => right
-  | .pair cf cg => pair (ofCode cf) (ofCode cg)
-  | .comp cf cg => comp (ofCode cf) (ofCode cg)
-  | .prec cf cg => prec (ofCode cf) (ofCode cg)
-  | .rfind' cf => rfind' (ofCode cf)
+  | .pair cf cg => pair (ofPartrecCode cf) (ofPartrecCode cg)
+  | .comp cf cg => comp (ofPartrecCode cf) (ofPartrecCode cg)
+  | .prec cf cg => prec (ofPartrecCode cf) (ofPartrecCode cg)
+  | .rfind' cf => rfind' (ofPartrecCode cf)
 
-/-- The conversion from `Code` to `OCode` is injective. -/
-theorem ofCode_inj : Function.Injective ofCode := by
+/-- The conversion from `Code` to `Code` is injective. -/
+theorem ofPartrecCode_inj : Function.Injective ofPartrecCode := by
   intro a b
-  induction a generalizing b with cases b <;> grind [ofCode]
+  induction a generalizing b with cases b <;> grind [ofPartrecCode]
 
-instance instInhabited : Inhabited OCode :=
+instance instInhabited : Inhabited Code :=
   ⟨zero⟩
 
-/-- An `OCode` for the constant function outputting `n`. -/
-protected def const (n : ℕ) : OCode := ofCode (Code.const n)
+/-- An `Code` for the constant function outputting `n`. -/
+protected def const (n : ℕ) : Code := ofPartrecCode (Nat.Partrec.Code.const n)
 
-/-- `OCode.const` is injective. -/
-theorem const_inj : Function.Injective OCode.const :=
-  ofCode_inj.comp @Code.const_inj
+/-- `Code.const` is injective. -/
+theorem const_inj : Function.Injective Code.const :=
+  ofPartrecCode_inj.comp @Nat.Partrec.Code.const_inj
 
-/-- An `OCode` for the identity function. -/
-protected def id : OCode := ofCode Code.id
+/-- An `Code` for the identity function. -/
+protected def id : Code := ofPartrecCode Nat.Partrec.Code.id
 
 /-- Given a code `c` taking a pair as input, returns a code using `n` as the first argument to `c`.
 -/
-def curry (c : OCode) (n : ℕ) : OCode :=
-  comp c (pair (OCode.const n) OCode.id)
+def curry (c : Code) (n : ℕ) : Code :=
+  comp c (pair (Code.const n) Code.id)
 
-/-- An encoding of a `RecursiveIn.OCode` as a ℕ. -/
-def encodeOCode : OCode → ℕ
+/-- An encoding of a `RecursiveIn.Code` as a ℕ. -/
+def encodeCode : Code → ℕ
   | zero => 0
   | succ => 1
   | left => 2
   | right => 3
   | oracle => 4
-  | pair cf cg => 2 * (2 * Nat.pair (encodeOCode cf) (encodeOCode cg)) + 5
-  | comp cf cg => 2 * (2 * Nat.pair (encodeOCode cf) (encodeOCode cg) + 1) + 5
-  | prec cf cg => (2 * (2 * Nat.pair (encodeOCode cf) (encodeOCode cg)) + 1) + 5
-  | rfind' cf => (2 * (2 * encodeOCode cf + 1) + 1) + 5
+  | pair cf cg => 2 * (2 * Nat.pair (encodeCode cf) (encodeCode cg)) + 5
+  | comp cf cg => 2 * (2 * Nat.pair (encodeCode cf) (encodeCode cg) + 1) + 5
+  | prec cf cg => (2 * (2 * Nat.pair (encodeCode cf) (encodeCode cg)) + 1) + 5
+  | rfind' cf => (2 * (2 * encodeCode cf + 1) + 1) + 5
 
 /--
-A decoder for `RecursiveIn.OCode.encodeOCode`, taking any ℕ to the `RecursiveIn.OCode` it represents.
+A decoder for `RecursiveIn.Code.encodeCode`, taking any ℕ to the `RecursiveIn.Code` it represents.
 -/
-def ofNatOCode : ℕ → OCode
+def ofNatCode : ℕ → Code
   | 0 => zero
   | 1 => succ
   | 2 => left
@@ -146,73 +146,73 @@ def ofNatOCode : ℕ → OCode
     have _m1 : m.unpair.1 < n + 5 := lt_of_le_of_lt m.unpair_left_le hm
     have _m2 : m.unpair.2 < n + 5 := lt_of_le_of_lt m.unpair_right_le hm
     match n.bodd, n.div2.bodd with
-    | false, false => pair (ofNatOCode m.unpair.1) (ofNatOCode m.unpair.2)
-    | false, true => comp (ofNatOCode m.unpair.1) (ofNatOCode m.unpair.2)
-    | true, false => prec (ofNatOCode m.unpair.1) (ofNatOCode m.unpair.2)
-    | true, true => rfind' (ofNatOCode m)
+    | false, false => pair (ofNatCode m.unpair.1) (ofNatCode m.unpair.2)
+    | false, true => comp (ofNatCode m.unpair.1) (ofNatCode m.unpair.2)
+    | true, false => prec (ofNatCode m.unpair.1) (ofNatCode m.unpair.2)
+    | true, true => rfind' (ofNatCode m)
 
 set_option backward.privateInPublic true in
-/-- Proof that `RecursiveIn.OCode.ofNatOCode` is the inverse of `RecursiveIn.OCode.encodeOCode` -/
-private theorem encode_ofNatOCode : ∀ n, encodeOCode (ofNatOCode n) = n
-  | 0 => by simp [ofNatOCode, encodeOCode]
-  | 1 => by simp [ofNatOCode, encodeOCode]
-  | 2 => by simp [ofNatOCode, encodeOCode]
-  | 3 => by simp [ofNatOCode, encodeOCode]
-  | 4 => by simp [ofNatOCode, encodeOCode]
+/-- Proof that `RecursiveIn.Code.ofNatCode` is the inverse of `RecursiveIn.Code.encodeCode` -/
+private theorem encode_ofNatCode : ∀ n, encodeCode (ofNatCode n) = n
+  | 0 => by simp [ofNatCode, encodeCode]
+  | 1 => by simp [ofNatCode, encodeCode]
+  | 2 => by simp [ofNatCode, encodeCode]
+  | 3 => by simp [ofNatCode, encodeCode]
+  | 4 => by simp [ofNatCode, encodeCode]
   | n + 5 => by
     let m := n.div2.div2
     have hm : m < n + 5 := by grind
     have _m1 : m.unpair.1 < n + 5 := lt_of_le_of_lt m.unpair_left_le hm
     have _m2 : m.unpair.2 < n + 5 := lt_of_le_of_lt m.unpair_right_le hm
-    have IH := encode_ofNatOCode m
-    have IH1 := encode_ofNatOCode m.unpair.1
-    have IH2 := encode_ofNatOCode m.unpair.2
+    have IH := encode_ofNatCode m
+    have IH1 := encode_ofNatCode m.unpair.1
+    have IH2 := encode_ofNatCode m.unpair.2
     conv_rhs => rw [← Nat.bit_bodd_div2 n, ← Nat.bit_bodd_div2 n.div2]
-    simp only [ofNatOCode]
+    simp only [ofNatCode]
     cases n.bodd <;> cases n.div2.bodd <;>
-      simp [m, encodeOCode, IH, IH1, IH2, Nat.bit_val]
+      simp [m, encodeCode, IH, IH1, IH2, Nat.bit_val]
 
 set_option backward.privateInPublic true in
 set_option backward.privateInPublic.warn false in
-instance instDenumerable : Denumerable OCode :=
+instance instDenumerable : Denumerable Code :=
   mk'
-    ⟨encodeOCode, ofNatOCode, fun c => by
-        induction c <;> simp [encodeOCode, ofNatOCode, Nat.div2_val, *],
-      encode_ofNatOCode⟩
+    ⟨encodeCode, ofNatCode, fun c => by
+        induction c <;> simp [encodeCode, ofNatCode, Nat.div2_val, *],
+      encode_ofNatCode⟩
 
-theorem encodeOCode_eq : encode = encodeOCode :=
+theorem encodeCode_eq : encode = encodeCode :=
   rfl
 
-theorem ofNatOCode_eq : ofNat OCode = ofNatOCode :=
+theorem ofNatCode_eq : ofNat Code = ofNatCode :=
   rfl
 
 theorem encode_lt_pair (cf cg) :
     encode cf < encode (pair cf cg) ∧ encode cg < encode (pair cf cg) := by
-  simp only [encodeOCode_eq, encodeOCode]
-  have := Nat.mul_le_mul_right (Nat.pair cf.encodeOCode cg.encodeOCode) (by decide : 1 ≤ 2 * 2)
+  simp only [encodeCode_eq, encodeCode]
+  have := Nat.mul_le_mul_right (Nat.pair cf.encodeCode cg.encodeCode) (by decide : 1 ≤ 2 * 2)
   rw [one_mul, mul_assoc] at this
   have := lt_of_le_of_lt this (lt_add_of_pos_right _ (by decide : 0 < 5))
   exact ⟨lt_of_le_of_lt (Nat.left_le_pair _ _) this, lt_of_le_of_lt (Nat.right_le_pair _ _) this⟩
 
 theorem encode_lt_comp (cf cg) :
     encode cf < encode (comp cf cg) ∧ encode cg < encode (comp cf cg) := by
-  have : encode (pair cf cg) < encode (comp cf cg) := by simp [encodeOCode_eq, encodeOCode]
+  have : encode (pair cf cg) < encode (comp cf cg) := by simp [encodeCode_eq, encodeCode]
   exact (encode_lt_pair cf cg).imp (fun h => lt_trans h this) fun h => lt_trans h this
 
 theorem encode_lt_prec (cf cg) :
     encode cf < encode (prec cf cg) ∧ encode cg < encode (prec cf cg) := by
-  have : encode (pair cf cg) < encode (prec cf cg) := by simp [encodeOCode_eq, encodeOCode]
+  have : encode (pair cf cg) < encode (prec cf cg) := by simp [encodeCode_eq, encodeCode]
   exact (encode_lt_pair cf cg).imp (fun h => lt_trans h this) fun h => lt_trans h this
 
 theorem encode_lt_rfind' (cf) : encode cf < encode (rfind' cf) := by
-  simp only [encodeOCode_eq, encodeOCode]
+  simp only [encodeCode_eq, encodeCode]
   lia
 
-end RecursiveIn.OCode
+end RecursiveIn.Code
 
 section
 open Nat Primrec
-namespace RecursiveIn.OCode
+namespace RecursiveIn.Code
 
 theorem primrec₂_pair : Primrec₂ pair :=
   Primrec₂.ofNat_iff.2 <|
@@ -220,8 +220,8 @@ theorem primrec₂_pair : Primrec₂ pair :=
       nat_add.comp
         (nat_double.comp <|
           nat_double.comp <|
-            Primrec₂.natPair.comp (encode_iff.2 <| (Primrec.ofNat OCode).comp fst)
-              (encode_iff.2 <| (Primrec.ofNat OCode).comp snd))
+            Primrec₂.natPair.comp (encode_iff.2 <| (Primrec.ofNat Code).comp fst)
+              (encode_iff.2 <| (Primrec.ofNat Code).comp snd))
         (Primrec₂.const 5)
 
 theorem primrec₂_comp : Primrec₂ comp :=
@@ -230,8 +230,8 @@ theorem primrec₂_comp : Primrec₂ comp :=
       nat_add.comp
         (nat_double.comp <|
           nat_double_succ.comp <|
-            Primrec₂.natPair.comp (encode_iff.2 <| (Primrec.ofNat OCode).comp fst)
-              (encode_iff.2 <| (Primrec.ofNat OCode).comp snd))
+            Primrec₂.natPair.comp (encode_iff.2 <| (Primrec.ofNat Code).comp fst)
+              (encode_iff.2 <| (Primrec.ofNat Code).comp snd))
         (Primrec₂.const 5)
 
 theorem primrec₂_prec : Primrec₂ prec :=
@@ -240,8 +240,8 @@ theorem primrec₂_prec : Primrec₂ prec :=
       nat_add.comp
         (nat_double_succ.comp <|
           nat_double.comp <|
-            Primrec₂.natPair.comp (encode_iff.2 <| (Primrec.ofNat OCode).comp fst)
-              (encode_iff.2 <| (Primrec.ofNat OCode).comp snd))
+            Primrec₂.natPair.comp (encode_iff.2 <| (Primrec.ofNat Code).comp fst)
+              (encode_iff.2 <| (Primrec.ofNat Code).comp snd))
         (Primrec₂.const 5)
 
 theorem primrec_rfind' : Primrec rfind' :=
@@ -249,22 +249,22 @@ theorem primrec_rfind' : Primrec rfind' :=
     encode_iff.1 <|
       nat_add.comp
         (nat_double_succ.comp <| nat_double_succ.comp <|
-          encode_iff.2 <| Primrec.ofNat OCode)
+          encode_iff.2 <| Primrec.ofNat Code)
         (const 5)
 
 set_option linter.flexible false in -- TODO: revisit this after #13791 is merged
 theorem primrec_recOn' {α σ}
-    [Primcodable α] [Primcodable σ] {c : α → OCode} (hc : Primrec c) {z : α → σ}
+    [Primcodable α] [Primcodable σ] {c : α → Code} (hc : Primrec c) {z : α → σ}
     (hz : Primrec z) {s : α → σ} (hs : Primrec s) {l : α → σ} (hl : Primrec l) {r : α → σ}
-    (hr : Primrec r) {o : α → σ} (ho : Primrec o) {pr : α → OCode × OCode × σ × σ → σ} (hpr : Primrec₂ pr)
-    {co : α → OCode × OCode × σ × σ → σ} (hco : Primrec₂ co) {pc : α → OCode × OCode × σ × σ → σ}
-    (hpc : Primrec₂ pc) {rf : α → OCode × σ → σ} (hrf : Primrec₂ rf) :
+    (hr : Primrec r) {o : α → σ} (ho : Primrec o) {pr : α → Code × Code × σ × σ → σ} (hpr : Primrec₂ pr)
+    {co : α → Code × Code × σ × σ → σ} (hco : Primrec₂ co) {pc : α → Code × Code × σ × σ → σ}
+    (hpc : Primrec₂ pc) {rf : α → Code × σ → σ} (hrf : Primrec₂ rf) :
     let PR (a) cf cg hf hg := pr a (cf, cg, hf, hg)
     let CO (a) cf cg hf hg := co a (cf, cg, hf, hg)
     let PC (a) cf cg hf hg := pc a (cf, cg, hf, hg)
     let RF (a) cf hf := rf a (cf, hf)
-    let F (a : α) (c : OCode) : σ :=
-      RecursiveIn.OCode.recOn c (z a) (s a) (l a) (r a) (o a) (PR a) (CO a) (PC a) (RF a)
+    let F (a : α) (c : Code) : σ :=
+      RecursiveIn.Code.recOn c (z a) (s a) (l a) (r a) (o a) (PR a) (CO a) (PC a) (RF a)
     Primrec (fun a => F a (c a) : α → σ) := by
   intro _ _ _ _ F
   let G₁ : (α × List σ) × ℕ × ℕ → Option σ := fun p =>
@@ -273,10 +273,10 @@ theorem primrec_recOn' {α σ}
     IH[m.unpair.1]?.bind fun s₁ =>
     IH[m.unpair.2]?.map fun s₂ =>
     cond n.bodd
-      (cond n.div2.bodd (rf a (ofNat OCode m, s))
-        (pc a (ofNat OCode m.unpair.1, ofNat OCode m.unpair.2, s₁, s₂)))
-      (cond n.div2.bodd (co a (ofNat OCode m.unpair.1, ofNat OCode m.unpair.2, s₁, s₂))
-        (pr a (ofNat OCode m.unpair.1, ofNat OCode m.unpair.2, s₁, s₂)))
+      (cond n.div2.bodd (rf a (ofNat Code m, s))
+        (pc a (ofNat Code m.unpair.1, ofNat Code m.unpair.2, s₁, s₂)))
+      (cond n.div2.bodd (co a (ofNat Code m.unpair.1, ofNat Code m.unpair.2, s₁, s₂))
+        (pr a (ofNat Code m.unpair.1, ofNat Code m.unpair.2, s₁, s₂)))
   have : Primrec G₁ :=
     option_bind (list_getElem?.comp (snd.comp fst) (snd.comp snd)) <| .mk <|
     option_bind ((list_getElem?.comp (snd.comp fst)
@@ -293,14 +293,14 @@ theorem primrec_recOn' {α σ}
     have s₂ := snd
     (nat_bodd.comp n).cond
       ((nat_bodd.comp <| nat_div2.comp n).cond
-        (hrf.comp a (((Primrec.ofNat OCode).comp m).pair s))
-        (hpc.comp a (((Primrec.ofNat OCode).comp m₁).pair <|
-          ((Primrec.ofNat OCode).comp m₂).pair <| s₁.pair s₂)))
+        (hrf.comp a (((Primrec.ofNat Code).comp m).pair s))
+        (hpc.comp a (((Primrec.ofNat Code).comp m₁).pair <|
+          ((Primrec.ofNat Code).comp m₂).pair <| s₁.pair s₂)))
       (Primrec.cond (nat_bodd.comp <| nat_div2.comp n)
-        (hco.comp a (((Primrec.ofNat OCode).comp m₁).pair <|
-          ((Primrec.ofNat OCode).comp m₂).pair <| s₁.pair s₂))
-        (hpr.comp a (((Primrec.ofNat OCode).comp m₁).pair <|
-          ((Primrec.ofNat OCode).comp m₂).pair <| s₁.pair s₂)))
+        (hco.comp a (((Primrec.ofNat Code).comp m₁).pair <|
+          ((Primrec.ofNat Code).comp m₂).pair <| s₁.pair s₂))
+        (hpr.comp a (((Primrec.ofNat Code).comp m₁).pair <|
+          ((Primrec.ofNat Code).comp m₂).pair <| s₁.pair s₂)))
   let G : α → List σ → Option σ := fun a IH =>
     IH.length.casesOn (some (z a)) fun n =>
     n.casesOn (some (s a)) fun n =>
@@ -317,13 +317,13 @@ theorem primrec_recOn' {α σ}
     this.comp <|
       ((fst.pair snd).comp <| fst.comp <| fst.comp <| fst.comp <| fst.comp <| fst).pair <|
       snd.pair <| nat_div2.comp <| nat_div2.comp snd
-  refine (nat_strong_rec (fun a n => F a (ofNat OCode n)) this.to₂ fun a n => ?_)
+  refine (nat_strong_rec (fun a n => F a (ofNat Code n)) this.to₂ fun a n => ?_)
     |>.comp .id (encode_iff.2 hc) |>.of_eq fun a => by simp
-  iterate 5 rcases n with - | n; · simp [ofNatOCode_eq, ofNatOCode]; rfl
+  iterate 5 rcases n with - | n; · simp [ofNatCode_eq, ofNatCode]; rfl
   simp only [G]; rw [List.length_map, List.length_range]
   let m := n.div2.div2
-  change G₁ ((a, (List.range (n + 5)).map fun n => F a (ofNat OCode n)), n, m)
-    = some (F a (ofNat OCode (n + 5)))
+  change G₁ ((a, (List.range (n + 5)).map fun n => F a (ofNat Code n)), n, m)
+    = some (F a (ofNat Code (n + 5)))
   have hm : m < n + 5 := by
     simp only [m, div2_val]
     exact lt_of_le_of_lt
@@ -332,23 +332,23 @@ theorem primrec_recOn' {α σ}
   have m1 : m.unpair.1 < n + 5 := lt_of_le_of_lt m.unpair_left_le hm
   have m2 : m.unpair.2 < n + 5 := lt_of_le_of_lt m.unpair_right_le hm
   simp [G₁, m, hm, m1, m2]
-  rw [show ofNat OCode (n + 5) = ofNatOCode (n + 5) from rfl]
-  simp [ofNatOCode]
+  rw [show ofNat Code (n + 5) = ofNatCode (n + 5) from rfl]
+  simp [ofNatCode]
   cases n.bodd <;> cases n.div2.bodd <;> rfl
 
-/-- Recursion on `RecursiveIn.OCode` is primitive recursive. -/
+/-- Recursion on `RecursiveIn.Code` is primitive recursive. -/
 theorem primrec_recOn {α σ}
-    [Primcodable α] [Primcodable σ] {c : α → OCode} (hc : Primrec c) {z : α → σ}
+    [Primcodable α] [Primcodable σ] {c : α → Code} (hc : Primrec c) {z : α → σ}
     (hz : Primrec z) {s : α → σ} (hs : Primrec s) {l : α → σ} (hl : Primrec l) {r : α → σ}
-    (hr : Primrec r) {o : α → σ} (ho : Primrec o) {pr : α → OCode → OCode → σ → σ → σ}
-    (hpr : Primrec fun a : α × OCode × OCode × σ × σ => pr a.1 a.2.1 a.2.2.1 a.2.2.2.1 a.2.2.2.2)
-    {co : α → OCode → OCode → σ → σ → σ}
-    (hco : Primrec fun a : α × OCode × OCode × σ × σ => co a.1 a.2.1 a.2.2.1 a.2.2.2.1 a.2.2.2.2)
-    {pc : α → OCode → OCode → σ → σ → σ}
-    (hpc : Primrec fun a : α × OCode × OCode × σ × σ => pc a.1 a.2.1 a.2.2.1 a.2.2.2.1 a.2.2.2.2)
-    {rf : α → OCode → σ → σ} (hrf : Primrec fun a : α × OCode × σ => rf a.1 a.2.1 a.2.2) :
-    let F (a : α) (c : OCode) : σ :=
-      RecursiveIn.OCode.recOn c (z a) (s a) (l a) (r a) (o a) (pr a) (co a) (pc a) (rf a)
+    (hr : Primrec r) {o : α → σ} (ho : Primrec o) {pr : α → Code → Code → σ → σ → σ}
+    (hpr : Primrec fun a : α × Code × Code × σ × σ => pr a.1 a.2.1 a.2.2.1 a.2.2.2.1 a.2.2.2.2)
+    {co : α → Code → Code → σ → σ → σ}
+    (hco : Primrec fun a : α × Code × Code × σ × σ => co a.1 a.2.1 a.2.2.1 a.2.2.2.1 a.2.2.2.2)
+    {pc : α → Code → Code → σ → σ → σ}
+    (hpc : Primrec fun a : α × Code × Code × σ × σ => pc a.1 a.2.1 a.2.2.1 a.2.2.2.1 a.2.2.2.2)
+    {rf : α → Code → σ → σ} (hrf : Primrec fun a : α × Code × σ => rf a.1 a.2.1 a.2.2) :
+    let F (a : α) (c : Code) : σ :=
+      RecursiveIn.Code.recOn c (z a) (s a) (l a) (r a) (o a) (pr a) (co a) (pc a) (rf a)
     Primrec fun a => F a (c a) :=
   primrec_recOn' hc hz hs hl hr ho
     (pr := fun a b => pr a b.1 b.2.1 b.2.2.1 b.2.2.2) (.mk hpr)
@@ -356,27 +356,27 @@ theorem primrec_recOn {α σ}
     (pc := fun a b => pc a b.1 b.2.1 b.2.2.1 b.2.2.2) (.mk hpc)
     (rf := fun a b => rf a b.1 b.2) (.mk hrf)
 
-end RecursiveIn.OCode
+end RecursiveIn.Code
 end
 
-namespace RecursiveIn.OCode
+namespace RecursiveIn.Code
 section
 
 open Nat Computable
 
 set_option linter.flexible false in -- TODO: revisit this after #13791 is merged
-/-- Recursion on `RecursiveIn.OCode` is computable. -/
-theorem computable_recOn {α σ} [Primcodable α] [Primcodable σ] {c : α → OCode} (hc : Computable c)
+/-- Recursion on `RecursiveIn.Code` is computable. -/
+theorem computable_recOn {α σ} [Primcodable α] [Primcodable σ] {c : α → Code} (hc : Computable c)
     {z : α → σ} (hz : Computable z) {s : α → σ} (hs : Computable s) {l : α → σ} (hl : Computable l)
-    {r : α → σ} (hr : Computable r) {o : α → σ} (ho : Computable o) {pr : α → OCode × OCode × σ × σ → σ} (hpr : Computable₂ pr)
-    {co : α → OCode × OCode × σ × σ → σ} (hco : Computable₂ co) {pc : α → OCode × OCode × σ × σ → σ}
-    (hpc : Computable₂ pc) {rf : α → OCode × σ → σ} (hrf : Computable₂ rf) :
+    {r : α → σ} (hr : Computable r) {o : α → σ} (ho : Computable o) {pr : α → Code × Code × σ × σ → σ} (hpr : Computable₂ pr)
+    {co : α → Code × Code × σ × σ → σ} (hco : Computable₂ co) {pc : α → Code × Code × σ × σ → σ}
+    (hpc : Computable₂ pc) {rf : α → Code × σ → σ} (hrf : Computable₂ rf) :
     let PR (a) cf cg hf hg := pr a (cf, cg, hf, hg)
     let CO (a) cf cg hf hg := co a (cf, cg, hf, hg)
     let PC (a) cf cg hf hg := pc a (cf, cg, hf, hg)
     let RF (a) cf hf := rf a (cf, hf)
-    let F (a : α) (c : OCode) : σ :=
-      RecursiveIn.OCode.recOn c (z a) (s a) (l a) (r a) (o a) (PR a) (CO a) (PC a) (RF a)
+    let F (a : α) (c : Code) : σ :=
+      RecursiveIn.Code.recOn c (z a) (s a) (l a) (r a) (o a) (PR a) (CO a) (PC a) (RF a)
     Computable fun a => F a (c a) := by
   intro _ _ _ _ F
   let G₁ : (α × List σ) × ℕ × ℕ → Option σ := fun p =>
@@ -385,10 +385,10 @@ theorem computable_recOn {α σ} [Primcodable α] [Primcodable σ] {c : α → O
     IH[m.unpair.1]?.bind fun s₁ =>
     IH[m.unpair.2]?.map fun s₂ =>
     cond n.bodd
-      (cond n.div2.bodd (rf a (ofNat OCode m, s))
-        (pc a (ofNat OCode m.unpair.1, ofNat OCode m.unpair.2, s₁, s₂)))
-      (cond n.div2.bodd (co a (ofNat OCode m.unpair.1, ofNat OCode m.unpair.2, s₁, s₂))
-        (pr a (ofNat OCode m.unpair.1, ofNat OCode m.unpair.2, s₁, s₂)))
+      (cond n.div2.bodd (rf a (ofNat Code m, s))
+        (pc a (ofNat Code m.unpair.1, ofNat Code m.unpair.2, s₁, s₂)))
+      (cond n.div2.bodd (co a (ofNat Code m.unpair.1, ofNat Code m.unpair.2, s₁, s₂))
+        (pr a (ofNat Code m.unpair.1, ofNat Code m.unpair.2, s₁, s₂)))
   have : Computable G₁ := by
     refine option_bind (list_getElem?.comp (snd.comp fst) (snd.comp snd)) <| .mk ?_
     refine option_bind ((list_getElem?.comp (snd.comp fst)
@@ -406,14 +406,14 @@ theorem computable_recOn {α σ} [Primcodable α] [Primcodable σ] {c : α → O
       have s₂ := snd
       (nat_bodd.comp n).cond
         ((nat_bodd.comp <| nat_div2.comp n).cond
-          (hrf.comp a (((Computable.ofNat OCode).comp m).pair s))
-          (hpc.comp a (((Computable.ofNat OCode).comp m₁).pair <|
-            ((Computable.ofNat OCode).comp m₂).pair <| s₁.pair s₂)))
+          (hrf.comp a (((Computable.ofNat Code).comp m).pair s))
+          (hpc.comp a (((Computable.ofNat Code).comp m₁).pair <|
+            ((Computable.ofNat Code).comp m₂).pair <| s₁.pair s₂)))
         (Computable.cond (nat_bodd.comp <| nat_div2.comp n)
-          (hco.comp a (((Computable.ofNat OCode).comp m₁).pair <|
-            ((Computable.ofNat OCode).comp m₂).pair <| s₁.pair s₂))
-          (hpr.comp a (((Computable.ofNat OCode).comp m₁).pair <|
-            ((Computable.ofNat OCode).comp m₂).pair <| s₁.pair s₂)))
+          (hco.comp a (((Computable.ofNat Code).comp m₁).pair <|
+            ((Computable.ofNat Code).comp m₂).pair <| s₁.pair s₂))
+          (hpr.comp a (((Computable.ofNat Code).comp m₁).pair <|
+            ((Computable.ofNat Code).comp m₂).pair <| s₁.pair s₂)))
   let G : α → List σ → Option σ := fun a IH =>
     IH.length.casesOn (some (z a)) fun n =>
     n.casesOn (some (s a)) fun n =>
@@ -430,13 +430,13 @@ theorem computable_recOn {α σ} [Primcodable α] [Primcodable σ] {c : α → O
     this.comp <|
       ((fst.pair snd).comp <| fst.comp <| fst.comp <| fst.comp <| fst.comp <| fst).pair <|
       snd.pair <| nat_div2.comp <| nat_div2.comp snd
-  refine (nat_strong_rec (fun a n => F a (ofNat OCode n)) this.to₂ fun a n => ?_)
+  refine (nat_strong_rec (fun a n => F a (ofNat Code n)) this.to₂ fun a n => ?_)
     |>.comp .id (encode_iff.2 hc) |>.of_eq fun a => by simp
-  iterate 5 rcases n with - | n; · simp [ofNatOCode_eq, ofNatOCode]; rfl
+  iterate 5 rcases n with - | n; · simp [ofNatCode_eq, ofNatCode]; rfl
   simp only [G]; rw [List.length_map, List.length_range]
   let m := n.div2.div2
-  change G₁ ((a, (List.range (n + 5)).map fun n => F a (ofNat OCode n)), n, m)
-    = some (F a (ofNat OCode (n + 5)))
+  change G₁ ((a, (List.range (n + 5)).map fun n => F a (ofNat Code n)), n, m)
+    = some (F a (ofNat Code (n + 5)))
   have hm : m < n + 5 := by
     simp only [m, div2_val]
     exact lt_of_le_of_lt
@@ -445,28 +445,28 @@ theorem computable_recOn {α σ} [Primcodable α] [Primcodable σ] {c : α → O
   have m1 : m.unpair.1 < n + 5 := lt_of_le_of_lt m.unpair_left_le hm
   have m2 : m.unpair.2 < n + 5 := lt_of_le_of_lt m.unpair_right_le hm
   simp [G₁, m, hm, m1, m2]
-  rw [show ofNat OCode (n + 5) = ofNatOCode (n + 5) from rfl]
-  simp [ofNatOCode]
+  rw [show ofNat Code (n + 5) = ofNatCode (n + 5) from rfl]
+  simp [ofNatCode]
   cases n.bodd <;> cases n.div2.bodd <;> rfl
 
 end
 
-/-- The interpretation of a `RecursiveIn.OCode` as a partial function.
-* `RecursiveIn.OCode.zero`: The constant zero function.
-* `RecursiveIn.OCode.succ`: The successor function.
-* `RecursiveIn.OCode.left`: Left unpairing of a pair of ℕ (encoded by `Nat.pair`)
-* `RecursiveIn.OCode.right`: Right unpairing of a pair of ℕ (encoded by `Nat.pair`)
-* `RecursiveIn.OCode.oracle`: The oracle function.
-* `RecursiveIn.OCode.pair`: Pairs the outputs of argument codes using `Nat.pair`.
-* `RecursiveIn.OCode.comp`: Composition of two argument codes.
-* `RecursiveIn.OCode.prec`: Primitive recursion. Given an argument of the form `Nat.pair a n`:
+/-- The interpretation of a `RecursiveIn.Code` as a partial function.
+* `RecursiveIn.Code.zero`: The constant zero function.
+* `RecursiveIn.Code.succ`: The successor function.
+* `RecursiveIn.Code.left`: Left unpairing of a pair of ℕ (encoded by `Nat.pair`)
+* `RecursiveIn.Code.right`: Right unpairing of a pair of ℕ (encoded by `Nat.pair`)
+* `RecursiveIn.Code.oracle`: The oracle function.
+* `RecursiveIn.Code.pair`: Pairs the outputs of argument codes using `Nat.pair`.
+* `RecursiveIn.Code.comp`: Composition of two argument codes.
+* `RecursiveIn.Code.prec`: Primitive recursion. Given an argument of the form `Nat.pair a n`:
   * If `n = 0`, returns `eval cf o a`.
   * If `n = succ k`, returns `eval cg o (pair a (pair k (eval o (prec cf cg) (pair a k))))`
-* `RecursiveIn.OCode.rfind'`: Minimization starting at a provided value. Given an argument of the
+* `RecursiveIn.Code.rfind'`: Minimization starting at a provided value. Given an argument of the
   form `Nat.pair a m`, returns the least `n ≥ m` such that `eval cf o (pair a n) = 0`, if such an `n`
   exists and if `eval cf o (pair a k)` terminates for all `m ≤ k ≤ n`.
 -/
-def eval (c : OCode) (o : ℕ →. ℕ) : ℕ →. ℕ := match c with
+def eval (c : Code) (o : ℕ →. ℕ) : ℕ →. ℕ := match c with
   | zero => pure 0
   | succ => Nat.succ
   | left => ↑fun n : ℕ => n.unpair.1
@@ -485,45 +485,45 @@ def eval (c : OCode) (o : ℕ →. ℕ) : ℕ →. ℕ := match c with
 
 /-- Helper lemma for the evaluation of `prec` in the base case. -/
 @[simp]
-theorem eval_prec_zero (cf cg : OCode) (o : ℕ →. ℕ) (a : ℕ) : eval (prec cf cg) o (Nat.pair a 0) = eval cf o a := by
+theorem eval_prec_zero (cf cg : Code) (o : ℕ →. ℕ) (a : ℕ) : eval (prec cf cg) o (Nat.pair a 0) = eval cf o a := by
   rw [eval, Nat.unpaired, Nat.unpair_pair]
   simp (config := { Lean.Meta.Simp.neutralConfig with proj := true }) only []
   rw [Nat.rec_zero]
 
 /-- Helper lemma for the evaluation of `prec` in the recursive case. -/
-theorem eval_prec_succ (cf cg : OCode) (o : ℕ →. ℕ) (a k : ℕ) :
+theorem eval_prec_succ (cf cg : Code) (o : ℕ →. ℕ) (a k : ℕ) :
     eval (prec cf cg) o (Nat.pair a (Nat.succ k)) =
       do {let ih ← eval (prec cf cg) o (Nat.pair a k); eval cg o (Nat.pair a (Nat.pair k ih))} := by
   rw [eval, Nat.unpaired, Part.bind_eq_bind, Nat.unpair_pair]
   simp
 
 /--
-Evaluation of `ofCode` does not depend on the oracle.
+Evaluation of `ofPartrecCode` does not depend on the oracle.
 -/
 @[simp]
-theorem eval_ofCode (c : Nat.Partrec.Code) (o : ℕ →. ℕ) : (OCode.ofCode c).eval o = c.eval := by
-  induction c with simp [ofCode, eval, Nat.Partrec.Code.eval, *]
+theorem eval_ofPartrecCode (c : Nat.Partrec.Code) (o : ℕ →. ℕ) : (Code.ofPartrecCode c).eval o = c.eval := by
+  induction c with simp [ofPartrecCode, eval, Nat.Partrec.Code.eval, *]
 
 @[simp]
-theorem eval_const : ∀ n m o, eval (OCode.const n) o m = Part.some n := by
-  simp [OCode.const]
+theorem eval_const : ∀ n m o, eval (Code.const n) o m = Part.some n := by
+  simp [Code.const]
 
 @[simp]
-theorem eval_id (n) : ∀ o, eval OCode.id o n = Part.some n := by
-  simp [OCode.id]
+theorem eval_id (n) : ∀ o, eval Code.id o n = Part.some n := by
+  simp [Code.id]
 
 @[simp]
 theorem eval_curry (c o n x) : eval (curry c n) o x = eval c o (Nat.pair n x) := by simp! [Seq.seq, curry]
 
-theorem primrec_const : Primrec OCode.const :=
+theorem primrec_const : Primrec Code.const :=
   (_root_.Primrec.id.nat_iterate (_root_.Primrec.const zero)
     (primrec₂_comp.comp (_root_.Primrec.const succ) Primrec.snd).to₂).of_eq
     fun n => by simp; induction n <;>
-      simp [*, Nat.Partrec.Code.const, OCode.const, OCode.ofCode, Function.iterate_succ', -Function.iterate_succ]
+      simp [*, Nat.Partrec.Code.const, Code.const, Code.ofPartrecCode, Function.iterate_succ', -Function.iterate_succ]
 
 theorem primrec₂_curry : Primrec₂ curry :=
   primrec₂_comp.comp Primrec.fst <| primrec₂_pair.comp (primrec_const.comp Primrec.snd)
-    (_root_.Primrec.const OCode.id)
+    (_root_.Primrec.const Code.id)
 
 theorem curry_inj {c₁ c₂ n₁ n₂} (h : curry c₁ n₁ = curry c₂ n₂) : c₁ = c₂ ∧ n₁ = n₂ :=
   ⟨by injection h, by
@@ -532,15 +532,15 @@ theorem curry_inj {c₁ c₂ n₁ n₂} (h : curry c₁ n₁ = curry c₂ n₂) 
     exact const_inj h₃⟩
 
 /--
-The relative $S_n^m$ theorem: There is a computable function, namely `RecursiveIn.OCode.curry`, that takes a
+The relative $S_n^m$ theorem: There is a computable function, namely `RecursiveIn.Code.curry`, that takes a
 program and a ℕ `n`, and returns a new program using `n` as the first argument.
 -/
 theorem smn :
-    ∃ f : OCode → ℕ → OCode, Computable₂ f ∧ ∀ c o n x, eval (f c n) o x = eval c o (Nat.pair n x) :=
+    ∃ f : Code → ℕ → Code, Computable₂ f ∧ ∀ c o n x, eval (f c n) o x = eval c o (Nat.pair n x) :=
   ⟨curry, Primrec₂.to_comp primrec₂_curry, eval_curry⟩
 
-/-- A function `f` is Turing reducible to `g` if and only if there is an `OCode` which evaluates to `f`, given oracle `g`. -/
-theorem exists_code {f g : ℕ →. ℕ} : TuringReducible f g ↔ ∃ c : OCode, eval c g = f := by
+/-- A function `f` is Turing reducible to `g` if and only if there is an `Code` which evaluates to `f`, given oracle `g`. -/
+theorem exists_code {f g : ℕ →. ℕ} : TuringReducible f g ↔ ∃ c : Code, eval c g = f := by
   refine ⟨fun h => ?_, ?_⟩
   · induction h with
     | zero => exact ⟨zero, rfl⟩
@@ -559,7 +559,7 @@ theorem exists_code {f g : ℕ →. ℕ} : TuringReducible f g ↔ ∃ c : OCode
       exact ⟨prec cf cg, rfl⟩
     | rfind pf hf =>
       rcases hf with ⟨cf, rfl⟩
-      refine ⟨comp (rfind' cf) (pair OCode.id zero), ?_⟩
+      refine ⟨comp (rfind' cf) (pair Code.id zero), ?_⟩
       simp [eval, Seq.seq, pure, PFun.pure, Part.map_id']
   · rintro ⟨c, rfl⟩
     induction c with
@@ -573,11 +573,11 @@ theorem exists_code {f g : ℕ →. ℕ} : TuringReducible f g ↔ ∃ c : OCode
     | prec cf cg pf pg => exact pf.prec pg
     | rfind' cf pf => exact pf.rfind'
 
-/-- A modified evaluation for an `OCode` which returns an `Option ℕ` instead of a `Part ℕ`. To avoid undecidability, `evaln` takes a parameter `k` and fails if it encounters a number ≥ k in the course of its execution. Moreover, the provided oracle must be a function `ℕ → Option ℕ` rather than a function `ℕ →. ℕ`. Other than this, the semantics are the same as in `RecursiveIn.OCode.eval`.
+/-- A modified evaluation for an `Code` which returns an `Option ℕ` instead of a `Part ℕ`. To avoid undecidability, `evaln` takes a parameter `k` and fails if it encounters a number ≥ k in the course of its execution. Moreover, the provided oracle must be a function `ℕ → Option ℕ` rather than a function `ℕ →. ℕ`. Other than this, the semantics are the same as in `RecursiveIn.Code.eval`.
 
 TODO: Is using `ℕ → Option ℕ` as the oracle what we want here? Maybe we want to use `List ℕ` and `.get` instead. Then "`evaln` is primitive recursive" makes sense.
 -/
-def evaln : ℕ → OCode → (ℕ → Option ℕ) → ℕ → Option ℕ
+def evaln : ℕ → Code → (ℕ → Option ℕ) → ℕ → Option ℕ
   | 0, _ => fun _ _ => Option.none
   | k + 1, zero => fun _ n => do
     guard (n ≤ k)
@@ -628,155 +628,161 @@ theorem evaln_mono : ∀ {k₁ k₂ c g n x}, k₁ ≤ k₂ → x ∈ evaln k₁
   | 0, k₂, c, g, n, x, _, h => by simp [evaln] at h
   | k + 1, k₂ + 1, c, g, n, x, hl, h => by
     sorry
-    -- TODO: update this proof for OCode.
-    -- have hl' := Nat.le_of_succ_le_succ hl
-    -- have :
-    --   ∀ {k k₂ n x : ℕ} {o₁ o₂ : Option ℕ},
-    --     k ≤ k₂ → (x ∈ o₁ → x ∈ o₂) →
-    --       x ∈ do { guard (n ≤ k); o₁ } → x ∈ do { guard (n ≤ k₂); o₂ } := by
-    --   simp only [Option.mem_def, bind, Option.bind_eq_some_iff, Option.guard_eq_some',
-    --     exists_and_left, exists_const, and_imp]
-    --   introv h h₁ h₂ h₃
-    --   exact ⟨le_trans h₂ h, h₁ h₃⟩
-    -- simp? at h ⊢ says simp only [Option.mem_def] at h ⊢
-    -- induction c generalizing x n <;> rw [evaln] at h ⊢ <;> refine this hl' (fun h => ?_) h
-    -- iterate 4 exact h
-    -- case pair cf cg hf hg _ =>
-    --   simp? [Seq.seq, Option.bind_eq_some_iff] at h ⊢ says
-    --     simp only [Seq.seq, Option.map_eq_map, Option.mem_def, Option.bind_eq_some_iff,
-    --       Option.map_eq_some_iff, exists_exists_and_eq_and] at h ⊢
-    --   exact h.imp fun a => And.imp (hf _ _) <| Exists.imp fun b => And.imp_left (hg _ _)
-    -- case comp cf cg hf hg _ =>
-    --   simp? [Bind.bind, Option.bind_eq_some_iff] at h ⊢ says
-    --     simp only [bind, Option.mem_def, Option.bind_eq_some_iff] at h ⊢
-    --   exact h.imp fun a => And.imp (hg _ _) (hf _ _)
-    -- case prec cf cg hf hg _ =>
-    --   revert h
-    --   simp only [unpaired, bind, Option.mem_def]
-    --   induction n.unpair.2 <;> simp [Option.bind_eq_some_iff]
-    --   · apply hf
-    --   · exact fun y h₁ h₂ => ⟨y, evaln_mono hl' h₁, hg _ _ h₂⟩
-    -- case rfind' cf hf _ =>
-    --   simp? [Bind.bind, Option.bind_eq_some_iff] at h ⊢ says
-    --     simp only [unpaired, bind, pair_unpair, Option.pure_def, Option.mem_def,
-    --       Option.bind_eq_some_iff] at h ⊢
-    --   refine h.imp fun x => And.imp (hf _ _) ?_
-    --   by_cases x0 : x = 0 <;> simp [x0]
-    --   exact evaln_mono hl'
+    -- TODO: update this proof for RecursiveIn.Code.
+/-
+    have hl' := Nat.le_of_succ_le_succ hl
+    have :
+      ∀ {k k₂ n x : ℕ} {o₁ o₂ : Option ℕ},
+        k ≤ k₂ → (x ∈ o₁ → x ∈ o₂) →
+          x ∈ do { guard (n ≤ k); o₁ } → x ∈ do { guard (n ≤ k₂); o₂ } := by
+      simp only [Option.mem_def, bind, Option.bind_eq_some_iff, Option.guard_eq_some',
+        exists_and_left, exists_const, and_imp]
+      introv h h₁ h₂ h₃
+      exact ⟨le_trans h₂ h, h₁ h₃⟩
+    simp? at h ⊢ says simp only [Option.mem_def] at h ⊢
+    induction c generalizing x n <;> rw [evaln] at h ⊢ <;> refine this hl' (fun h => ?_) h
+    iterate 4 exact h
+    case pair cf cg hf hg _ =>
+      simp? [Seq.seq, Option.bind_eq_some_iff] at h ⊢ says
+        simp only [Seq.seq, Option.map_eq_map, Option.mem_def, Option.bind_eq_some_iff,
+          Option.map_eq_some_iff, exists_exists_and_eq_and] at h ⊢
+      exact h.imp fun a => And.imp (hf _ _) <| Exists.imp fun b => And.imp_left (hg _ _)
+    case comp cf cg hf hg _ =>
+      simp? [Bind.bind, Option.bind_eq_some_iff] at h ⊢ says
+        simp only [bind, Option.mem_def, Option.bind_eq_some_iff] at h ⊢
+      exact h.imp fun a => And.imp (hg _ _) (hf _ _)
+    case prec cf cg hf hg _ =>
+      revert h
+      simp only [unpaired, bind, Option.mem_def]
+      induction n.unpair.2 <;> simp [Option.bind_eq_some_iff]
+      · apply hf
+      · exact fun y h₁ h₂ => ⟨y, evaln_mono hl' h₁, hg _ _ h₂⟩
+    case rfind' cf hf _ =>
+      simp? [Bind.bind, Option.bind_eq_some_iff] at h ⊢ says
+        simp only [unpaired, bind, pair_unpair, Option.pure_def, Option.mem_def,
+          Option.bind_eq_some_iff] at h ⊢
+      refine h.imp fun x => And.imp (hf _ _) ?_
+      by_cases x0 : x = 0 <;> simp [x0]
+      exact evaln_mono hl'
+-/
 
 set_option linter.flexible false in -- TODO: revisit this after #13791 is merged
 -- TODO: Figure out the correct statement of this theorem.
--- theorem evaln_sound : ∀ {k c g n x}, x ∈ evaln k c g n → x ∈ eval c g n
---   | 0, _, g, n, x, h => by simp [evaln] at h
---   | k + 1, c, g, n, x, h => by
---     induction c generalizing x n <;> simp [eval, evaln, Option.bind_eq_some_iff, Seq.seq] at h ⊢ <;>
---       obtain ⟨_, h⟩ := h
---     iterate 4 simpa [pure, PFun.pure, eq_comm] using h
---     case pair cf cg hf hg _ =>
---       rcases h with ⟨y, ef, z, eg, rfl⟩
---       exact ⟨_, hf _ _ ef, _, hg _ _ eg, rfl⟩
---     case comp cf cg hf hg _ =>
---       rcases h with ⟨y, eg, ef⟩
---       exact ⟨_, hg _ _ eg, hf _ _ ef⟩
---     case prec cf cg hf hg _ =>
---       revert h
---       induction n.unpair.2 generalizing x with simp [Option.bind_eq_some_iff]
---       | zero => apply hf
---       | succ m IH =>
---         refine fun y h₁ h₂ => ⟨y, IH _ ?_, ?_⟩
---         · have := evaln_mono k.le_succ h₁
---           simp [evaln, Option.bind_eq_some_iff] at this
---           exact this.2
---         · exact hg _ _ h₂
---     case rfind' cf hf _ =>
---       rcases h with ⟨m, h₁, h₂⟩
---       by_cases m0 : m = 0 <;> simp [m0] at h₂
---       · exact
---           ⟨0, ⟨by simpa [m0] using hf _ _ h₁, fun {m} => (Nat.not_lt_zero _).elim⟩, by simp [h₂]⟩
---       · have := evaln_sound h₂
---         simp [eval] at this
---         rcases this with ⟨y, ⟨hy₁, hy₂⟩, rfl⟩
---         refine
---           ⟨y + 1, ⟨by simpa [add_comm, add_left_comm] using hy₁, fun {i} im => ?_⟩, by
---             simp [add_comm, add_left_comm]⟩
---         rcases i with - | i
---         · exact ⟨m, by simpa using hf _ _ h₁, m0⟩
---         · rcases hy₂ (Nat.lt_of_succ_lt_succ im) with ⟨z, hz, z0⟩
---           exact ⟨z, by simpa [add_comm, add_left_comm] using hz, z0⟩
+/-
+theorem evaln_sound : ∀ {k c g n x}, x ∈ evaln k c g n → x ∈ eval c g n
+  | 0, _, g, n, x, h => by simp [evaln] at h
+  | k + 1, c, g, n, x, h => by
+    induction c generalizing x n <;> simp [eval, evaln, Option.bind_eq_some_iff, Seq.seq] at h ⊢ <;>
+      obtain ⟨_, h⟩ := h
+    iterate 4 simpa [pure, PFun.pure, eq_comm] using h
+    case pair cf cg hf hg _ =>
+      rcases h with ⟨y, ef, z, eg, rfl⟩
+      exact ⟨_, hf _ _ ef, _, hg _ _ eg, rfl⟩
+    case comp cf cg hf hg _ =>
+      rcases h with ⟨y, eg, ef⟩
+      exact ⟨_, hg _ _ eg, hf _ _ ef⟩
+    case prec cf cg hf hg _ =>
+      revert h
+      induction n.unpair.2 generalizing x with simp [Option.bind_eq_some_iff]
+      | zero => apply hf
+      | succ m IH =>
+        refine fun y h₁ h₂ => ⟨y, IH _ ?_, ?_⟩
+        · have := evaln_mono k.le_succ h₁
+          simp [evaln, Option.bind_eq_some_iff] at this
+          exact this.2
+        · exact hg _ _ h₂
+    case rfind' cf hf _ =>
+      rcases h with ⟨m, h₁, h₂⟩
+      by_cases m0 : m = 0 <;> simp [m0] at h₂
+      · exact
+          ⟨0, ⟨by simpa [m0] using hf _ _ h₁, fun {m} => (Nat.not_lt_zero _).elim⟩, by simp [h₂]⟩
+      · have := evaln_sound h₂
+        simp [eval] at this
+        rcases this with ⟨y, ⟨hy₁, hy₂⟩, rfl⟩
+        refine
+          ⟨y + 1, ⟨by simpa [add_comm, add_left_comm] using hy₁, fun {i} im => ?_⟩, by
+            simp [add_comm, add_left_comm]⟩
+        rcases i with - | i
+        · exact ⟨m, by simpa using hf _ _ h₁, m0⟩
+        · rcases hy₂ (Nat.lt_of_succ_lt_succ im) with ⟨z, hz, z0⟩
+          exact ⟨z, by simpa [add_comm, add_left_comm] using hz, z0⟩
+-/
 
 set_option linter.flexible false in -- TODO: revisit this after #13791 is merged
 -- TODO: Figure out the correct statement of this theorem.
--- theorem evaln_complete {c g n x} : x ∈ eval c g n ↔ ∃ k, x ∈ evaln k c g n := by
---   refine ⟨fun h => ?_, fun ⟨k, h⟩ => evaln_sound h⟩
---   rsuffices ⟨k, h⟩ : ∃ k, x ∈ evaln (k + 1) c n
---   · exact ⟨k + 1, h⟩
---   induction c generalizing n x with
---       simp [eval, evaln, pure, PFun.pure, Seq.seq, Option.bind_eq_some_iff] at h ⊢
---   | pair cf cg hf hg =>
---     rcases h with ⟨x, hx, y, hy, rfl⟩
---     rcases hf hx with ⟨k₁, hk₁⟩; rcases hg hy with ⟨k₂, hk₂⟩
---     refine ⟨max k₁ k₂, ?_⟩
---     refine
---       ⟨le_max_of_le_left <| Nat.le_of_lt_succ <| evaln_bound hk₁, _,
---         evaln_mono (Nat.succ_le_succ <| le_max_left _ _) hk₁, _,
---         evaln_mono (Nat.succ_le_succ <| le_max_right _ _) hk₂, rfl⟩
---   | comp cf cg hf hg =>
---     rcases h with ⟨y, hy, hx⟩
---     rcases hg hy with ⟨k₁, hk₁⟩; rcases hf hx with ⟨k₂, hk₂⟩
---     refine ⟨max k₁ k₂, ?_⟩
---     exact
---       ⟨le_max_of_le_left <| Nat.le_of_lt_succ <| evaln_bound hk₁, _,
---         evaln_mono (Nat.succ_le_succ <| le_max_left _ _) hk₁,
---         evaln_mono (Nat.succ_le_succ <| le_max_right _ _) hk₂⟩
---   | prec cf cg hf hg =>
---     revert h
---     generalize n.unpair.1 = n₁; generalize n.unpair.2 = n₂
---     induction n₂ generalizing x n with simp [Option.bind_eq_some_iff]
---     | zero =>
---       intro h
---       rcases hf h with ⟨k, hk⟩
---       exact ⟨_, le_max_left _ _, evaln_mono (Nat.succ_le_succ <| le_max_right _ _) hk⟩
---     | succ m IH =>
---       intro y hy hx
---       rcases IH hy with ⟨k₁, nk₁, hk₁⟩
---       rcases hg hx with ⟨k₂, hk₂⟩
---       refine
---         ⟨(max k₁ k₂).succ,
---           Nat.le_succ_of_le <| le_max_of_le_left <|
---             le_trans (le_max_left _ (Nat.pair n₁ m)) nk₁, y,
---           evaln_mono (Nat.succ_le_succ <| le_max_left _ _) ?_,
---           evaln_mono (Nat.succ_le_succ <| Nat.le_succ_of_le <| le_max_right _ _) hk₂⟩
---       simp only [evaln.eq_8, bind, unpaired, unpair_pair, Option.mem_def, Option.bind_eq_some_iff,
---         Option.guard_eq_some', exists_and_left, exists_const]
---       exact ⟨le_trans (le_max_right _ _) nk₁, hk₁⟩
---   | rfind' cf hf =>
---     rcases h with ⟨y, ⟨hy₁, hy₂⟩, rfl⟩
---     suffices ∃ k, y + n.unpair.2 ∈ evaln (k + 1) (rfind' cf) (Nat.pair n.unpair.1 n.unpair.2) by
---       simpa [evaln, Option.bind_eq_some_iff]
---     revert hy₁ hy₂
---     generalize n.unpair.2 = m
---     intro hy₁ hy₂
---     induction y generalizing m with simp [evaln, Option.bind_eq_some_iff]
---     | zero =>
---       simp at hy₁
---       rcases hf hy₁ with ⟨k, hk⟩
---       exact ⟨_, Nat.le_of_lt_succ <| evaln_bound hk, _, hk, by simp⟩
---     | succ y IH =>
---       rcases hy₂ (Nat.succ_pos _) with ⟨a, ha, a0⟩
---       rcases hf ha with ⟨k₁, hk₁⟩
---       rcases IH m.succ (by simpa [Nat.succ_eq_add_one, add_comm, add_left_comm] using hy₁)
---           fun {i} hi => by
---           simpa [Nat.succ_eq_add_one, add_comm, add_left_comm] using
---             hy₂ (Nat.succ_lt_succ hi) with
---         ⟨k₂, hk₂⟩
---       use (max k₁ k₂).succ
---       rw [zero_add] at hk₁
---       use Nat.le_succ_of_le <| le_max_of_le_left <| Nat.le_of_lt_succ <| evaln_bound hk₁
---       use a
---       use evaln_mono (Nat.succ_le_succ <| Nat.le_succ_of_le <| le_max_left _ _) hk₁
---       simpa [a0, add_comm, add_left_comm] using
---         evaln_mono (Nat.succ_le_succ <| le_max_right _ _) hk₂
---   | _ => exact ⟨⟨_, le_rfl⟩, h.symm⟩
+/-
+theorem evaln_complete {c g n x} : x ∈ eval c g n ↔ ∃ k, x ∈ evaln k c g n := by
+  refine ⟨fun h => ?_, fun ⟨k, h⟩ => evaln_sound h⟩
+  rsuffices ⟨k, h⟩ : ∃ k, x ∈ evaln (k + 1) c n
+  · exact ⟨k + 1, h⟩
+  induction c generalizing n x with
+      simp [eval, evaln, pure, PFun.pure, Seq.seq, Option.bind_eq_some_iff] at h ⊢
+  | pair cf cg hf hg =>
+    rcases h with ⟨x, hx, y, hy, rfl⟩
+    rcases hf hx with ⟨k₁, hk₁⟩; rcases hg hy with ⟨k₂, hk₂⟩
+    refine ⟨max k₁ k₂, ?_⟩
+    refine
+      ⟨le_max_of_le_left <| Nat.le_of_lt_succ <| evaln_bound hk₁, _,
+        evaln_mono (Nat.succ_le_succ <| le_max_left _ _) hk₁, _,
+        evaln_mono (Nat.succ_le_succ <| le_max_right _ _) hk₂, rfl⟩
+  | comp cf cg hf hg =>
+    rcases h with ⟨y, hy, hx⟩
+    rcases hg hy with ⟨k₁, hk₁⟩; rcases hf hx with ⟨k₂, hk₂⟩
+    refine ⟨max k₁ k₂, ?_⟩
+    exact
+      ⟨le_max_of_le_left <| Nat.le_of_lt_succ <| evaln_bound hk₁, _,
+        evaln_mono (Nat.succ_le_succ <| le_max_left _ _) hk₁,
+        evaln_mono (Nat.succ_le_succ <| le_max_right _ _) hk₂⟩
+  | prec cf cg hf hg =>
+    revert h
+    generalize n.unpair.1 = n₁; generalize n.unpair.2 = n₂
+    induction n₂ generalizing x n with simp [Option.bind_eq_some_iff]
+    | zero =>
+      intro h
+      rcases hf h with ⟨k, hk⟩
+      exact ⟨_, le_max_left _ _, evaln_mono (Nat.succ_le_succ <| le_max_right _ _) hk⟩
+    | succ m IH =>
+      intro y hy hx
+      rcases IH hy with ⟨k₁, nk₁, hk₁⟩
+      rcases hg hx with ⟨k₂, hk₂⟩
+      refine
+        ⟨(max k₁ k₂).succ,
+          Nat.le_succ_of_le <| le_max_of_le_left <|
+            le_trans (le_max_left _ (Nat.pair n₁ m)) nk₁, y,
+          evaln_mono (Nat.succ_le_succ <| le_max_left _ _) ?_,
+          evaln_mono (Nat.succ_le_succ <| Nat.le_succ_of_le <| le_max_right _ _) hk₂⟩
+      simp only [evaln.eq_8, bind, unpaired, unpair_pair, Option.mem_def, Option.bind_eq_some_iff,
+        Option.guard_eq_some', exists_and_left, exists_const]
+      exact ⟨le_trans (le_max_right _ _) nk₁, hk₁⟩
+  | rfind' cf hf =>
+    rcases h with ⟨y, ⟨hy₁, hy₂⟩, rfl⟩
+    suffices ∃ k, y + n.unpair.2 ∈ evaln (k + 1) (rfind' cf) (Nat.pair n.unpair.1 n.unpair.2) by
+      simpa [evaln, Option.bind_eq_some_iff]
+    revert hy₁ hy₂
+    generalize n.unpair.2 = m
+    intro hy₁ hy₂
+    induction y generalizing m with simp [evaln, Option.bind_eq_some_iff]
+    | zero =>
+      simp at hy₁
+      rcases hf hy₁ with ⟨k, hk⟩
+      exact ⟨_, Nat.le_of_lt_succ <| evaln_bound hk, _, hk, by simp⟩
+    | succ y IH =>
+      rcases hy₂ (Nat.succ_pos _) with ⟨a, ha, a0⟩
+      rcases hf ha with ⟨k₁, hk₁⟩
+      rcases IH m.succ (by simpa [Nat.succ_eq_add_one, add_comm, add_left_comm] using hy₁)
+          fun {i} hi => by
+          simpa [Nat.succ_eq_add_one, add_comm, add_left_comm] using
+            hy₂ (Nat.succ_lt_succ hi) with
+        ⟨k₂, hk₂⟩
+      use (max k₁ k₂).succ
+      rw [zero_add] at hk₁
+      use Nat.le_succ_of_le <| le_max_of_le_left <| Nat.le_of_lt_succ <| evaln_bound hk₁
+      use a
+      use evaln_mono (Nat.succ_le_succ <| Nat.le_succ_of_le <| le_max_left _ _) hk₁
+      simpa [a0, add_comm, add_left_comm] using
+        evaln_mono (Nat.succ_le_succ <| le_max_right _ _) hk₂
+  | _ => exact ⟨⟨_, le_rfl⟩, h.symm⟩
+-/
 
 section
 
@@ -786,7 +792,7 @@ open Primrec
 TODO: Figure out what is going on in this section. What is `G` supposed to be? What are `lup` and `hlup` doing?
 -/
 
-private def lup (L : List (List (Option ℕ))) (p : ℕ × OCode) (n : ℕ) := do
+private def lup (L : List (List (Option ℕ))) (p : ℕ × Code) (n : ℕ) := do
   let l ← L[encode p]?
   let o ← l[n]?
   o
@@ -799,12 +805,12 @@ private theorem hlup : Primrec fun p : _ × (_ × _) × _ => lup p.1 p.2.1 p.2.2
 
 private def G (L : List (List (Option ℕ))) : Option (List (Option ℕ)) :=
   Option.some <|
-    let a := ofNat (ℕ × OCode) L.length
+    let a := ofNat (ℕ × Code) L.length
     let k := a.1
     let c := a.2
     (List.range k).map fun n =>
       k.casesOn Option.none fun k' =>
-        RecursiveIn.OCode.recOn c
+        RecursiveIn.Code.recOn c
           (some 0) -- zero
           (some (Nat.succ n))
           (some n.unpair.1)
@@ -832,181 +838,187 @@ private def G (L : List (List (Option ℕ))) : Option (List (Option ℕ)) :=
 private theorem hG : Primrec G := by
   sorry
   -- TODO: Update this proof? What is it doing?
-  -- have a := (Primrec.ofNat (ℕ × Code)).comp (Primrec.list_length (α := List (Option ℕ)))
-  -- have k := Primrec.fst.comp a
-  -- refine Primrec.option_some.comp (Primrec.list_map (Primrec.list_range.comp k) (?_ : Primrec _))
-  -- replace k := k.comp (Primrec.fst (β := ℕ))
-  -- have n := Primrec.snd (α := List (List (Option ℕ))) (β := ℕ)
-  -- refine Primrec.nat_casesOn k (_root_.Primrec.const Option.none) (?_ : Primrec _)
-  -- have k := k.comp (Primrec.fst (β := ℕ))
-  -- have n := n.comp (Primrec.fst (β := ℕ))
-  -- have k' := Primrec.snd (α := List (List (Option ℕ)) × ℕ) (β := ℕ)
-  -- have c := Primrec.snd.comp (a.comp <| (Primrec.fst (β := ℕ)).comp (Primrec.fst (β := ℕ)))
-  -- apply
-  --   Nat.Partrec.Code.primrec_recOn c
-  --     (_root_.Primrec.const (some 0))
-  --     (Primrec.option_some.comp (_root_.Primrec.succ.comp n))
-  --     (Primrec.option_some.comp (Primrec.fst.comp <| Primrec.unpair.comp n))
-  --     (Primrec.option_some.comp (Primrec.snd.comp <| Primrec.unpair.comp n))
-  -- · have L := (Primrec.fst.comp Primrec.fst).comp
-  --     (Primrec.fst (α := (List (List (Option ℕ)) × ℕ) × ℕ)
-  --       (β := Code × Code × Option ℕ × Option ℕ))
-  --   have k := k.comp (Primrec.fst (β := Code × Code × Option ℕ × Option ℕ))
-  --   have n := n.comp (Primrec.fst (β := Code × Code × Option ℕ × Option ℕ))
-  --   have cf := Primrec.fst.comp (Primrec.snd (α := (List (List (Option ℕ)) × ℕ) × ℕ)
-  --       (β := Code × Code × Option ℕ × Option ℕ))
-  --   have cg := (Primrec.fst.comp Primrec.snd).comp
-  --     (Primrec.snd (α := (List (List (Option ℕ)) × ℕ) × ℕ)
-  --       (β := Code × Code × Option ℕ × Option ℕ))
-  --   refine Primrec.option_bind (hlup.comp <| L.pair <| (k.pair cf).pair n) ?_
-  --   unfold Primrec₂
-  --   conv =>
-  --     congr
-  --     · ext p
-  --       dsimp only []
-  --       erw [Option.bind_eq_bind, ← Option.map_eq_bind]
-  --   refine Primrec.option_map ((hlup.comp <| L.pair <| (k.pair cg).pair n).comp Primrec.fst) ?_
-  --   unfold Primrec₂
-  --   exact Primrec₂.natPair.comp (Primrec.snd.comp Primrec.fst) Primrec.snd
-  -- · have L := (Primrec.fst.comp Primrec.fst).comp
-  --     (Primrec.fst (α := (List (List (Option ℕ)) × ℕ) × ℕ)
-  --       (β := Code × Code × Option ℕ × Option ℕ))
-  --   have k := k.comp (Primrec.fst (β := Code × Code × Option ℕ × Option ℕ))
-  --   have n := n.comp (Primrec.fst (β := Code × Code × Option ℕ × Option ℕ))
-  --   have cf := Primrec.fst.comp (Primrec.snd (α := (List (List (Option ℕ)) × ℕ) × ℕ)
-  --       (β := Code × Code × Option ℕ × Option ℕ))
-  --   have cg := (Primrec.fst.comp Primrec.snd).comp
-  --     (Primrec.snd (α := (List (List (Option ℕ)) × ℕ) × ℕ)
-  --       (β := Code × Code × Option ℕ × Option ℕ))
-  --   refine Primrec.option_bind (hlup.comp <| L.pair <| (k.pair cg).pair n) ?_
-  --   unfold Primrec₂
-  --   have h :=
-  --     hlup.comp ((L.comp Primrec.fst).pair <| ((k.pair cf).comp Primrec.fst).pair Primrec.snd)
-  --   exact h
-  -- · have L := (Primrec.fst.comp Primrec.fst).comp
-  --     (Primrec.fst (α := (List (List (Option ℕ)) × ℕ) × ℕ)
-  --       (β := Code × Code × Option ℕ × Option ℕ))
-  --   have k := k.comp (Primrec.fst (β := Code × Code × Option ℕ × Option ℕ))
-  --   have n := n.comp (Primrec.fst (β := Code × Code × Option ℕ × Option ℕ))
-  --   have cf := Primrec.fst.comp (Primrec.snd (α := (List (List (Option ℕ)) × ℕ) × ℕ)
-  --       (β := Code × Code × Option ℕ × Option ℕ))
-  --   have cg := (Primrec.fst.comp Primrec.snd).comp
-  --     (Primrec.snd (α := (List (List (Option ℕ)) × ℕ) × ℕ)
-  --       (β := Code × Code × Option ℕ × Option ℕ))
-  --   have z := Primrec.fst.comp (Primrec.unpair.comp n)
-  --   refine
-  --     Primrec.nat_casesOn (Primrec.snd.comp (Primrec.unpair.comp n))
-  --       (hlup.comp <| L.pair <| (k.pair cf).pair z)
-  --       (?_ : Primrec _)
-  --   have L := L.comp (Primrec.fst (β := ℕ))
-  --   have z := z.comp (Primrec.fst (β := ℕ))
-  --   have y := Primrec.snd
-  --     (α := ((List (List (Option ℕ)) × ℕ) × ℕ) × Code × Code × Option ℕ × Option ℕ) (β := ℕ)
-  --   have h₁ := hlup.comp <| L.pair <| (((k'.pair c).comp Primrec.fst).comp Primrec.fst).pair
-  --     (Primrec₂.natPair.comp z y)
-  --   refine Primrec.option_bind h₁ (?_ : Primrec _)
-  --   have z := z.comp (Primrec.fst (β := ℕ))
-  --   have y := y.comp (Primrec.fst (β := ℕ))
-  --   have i := Primrec.snd
-  --     (α := (((List (List (Option ℕ)) × ℕ) × ℕ) × Code × Code × Option ℕ × Option ℕ) × ℕ)
-  --     (β := ℕ)
-  --   have h₂ := hlup.comp ((L.comp Primrec.fst).pair <|
-  --     ((k.pair cg).comp <| Primrec.fst.comp Primrec.fst).pair <|
-  --       Primrec₂.natPair.comp z <| Primrec₂.natPair.comp y i)
-  --   exact h₂
-  -- · have L := (Primrec.fst.comp Primrec.fst).comp
-  --     (Primrec.fst (α := (List (List (Option ℕ)) × ℕ) × ℕ)
-  --       (β := Code × Option ℕ))
-  --   have k := k.comp (Primrec.fst (β := Code × Option ℕ))
-  --   have n := n.comp (Primrec.fst (β := Code × Option ℕ))
-  --   have cf := Primrec.fst.comp (Primrec.snd (α := (List (List (Option ℕ)) × ℕ) × ℕ)
-  --       (β := Code × Option ℕ))
-  --   have z := Primrec.fst.comp (Primrec.unpair.comp n)
-  --   have m := Primrec.snd.comp (Primrec.unpair.comp n)
-  --   have h₁ := hlup.comp <| L.pair <| (k.pair cf).pair (Primrec₂.natPair.comp z m)
-  --   refine Primrec.option_bind h₁ (?_ : Primrec _)
-  --   have m := m.comp (Primrec.fst (β := ℕ))
-  --   refine Primrec.nat_casesOn Primrec.snd (Primrec.option_some.comp m) ?_
-  --   unfold Primrec₂
-  --   exact (hlup.comp ((L.comp Primrec.fst).pair <|
-  --     ((k'.pair c).comp <| Primrec.fst.comp Primrec.fst).pair
-  --       (Primrec₂.natPair.comp (z.comp Primrec.fst) (_root_.Primrec.succ.comp m)))).comp
-  --     Primrec.fst
+/-
+  have a := (Primrec.ofNat (ℕ × Code)).comp (Primrec.list_length (α := List (Option ℕ)))
+  have k := Primrec.fst.comp a
+  refine Primrec.option_some.comp (Primrec.list_map (Primrec.list_range.comp k) (?_ : Primrec _))
+  replace k := k.comp (Primrec.fst (β := ℕ))
+  have n := Primrec.snd (α := List (List (Option ℕ))) (β := ℕ)
+  refine Primrec.nat_casesOn k (_root_.Primrec.const Option.none) (?_ : Primrec _)
+  have k := k.comp (Primrec.fst (β := ℕ))
+  have n := n.comp (Primrec.fst (β := ℕ))
+  have k' := Primrec.snd (α := List (List (Option ℕ)) × ℕ) (β := ℕ)
+  have c := Primrec.snd.comp (a.comp <| (Primrec.fst (β := ℕ)).comp (Primrec.fst (β := ℕ)))
+  apply
+    Nat.Partrec.Code.primrec_recOn c
+      (_root_.Primrec.const (some 0))
+      (Primrec.option_some.comp (_root_.Primrec.succ.comp n))
+      (Primrec.option_some.comp (Primrec.fst.comp <| Primrec.unpair.comp n))
+      (Primrec.option_some.comp (Primrec.snd.comp <| Primrec.unpair.comp n))
+  · have L := (Primrec.fst.comp Primrec.fst).comp
+      (Primrec.fst (α := (List (List (Option ℕ)) × ℕ) × ℕ)
+        (β := Code × Code × Option ℕ × Option ℕ))
+    have k := k.comp (Primrec.fst (β := Code × Code × Option ℕ × Option ℕ))
+    have n := n.comp (Primrec.fst (β := Code × Code × Option ℕ × Option ℕ))
+    have cf := Primrec.fst.comp (Primrec.snd (α := (List (List (Option ℕ)) × ℕ) × ℕ)
+        (β := Code × Code × Option ℕ × Option ℕ))
+    have cg := (Primrec.fst.comp Primrec.snd).comp
+      (Primrec.snd (α := (List (List (Option ℕ)) × ℕ) × ℕ)
+        (β := Code × Code × Option ℕ × Option ℕ))
+    refine Primrec.option_bind (hlup.comp <| L.pair <| (k.pair cf).pair n) ?_
+    unfold Primrec₂
+    conv =>
+      congr
+      · ext p
+        dsimp only []
+        erw [Option.bind_eq_bind, ← Option.map_eq_bind]
+    refine Primrec.option_map ((hlup.comp <| L.pair <| (k.pair cg).pair n).comp Primrec.fst) ?_
+    unfold Primrec₂
+    exact Primrec₂.natPair.comp (Primrec.snd.comp Primrec.fst) Primrec.snd
+  · have L := (Primrec.fst.comp Primrec.fst).comp
+      (Primrec.fst (α := (List (List (Option ℕ)) × ℕ) × ℕ)
+        (β := Code × Code × Option ℕ × Option ℕ))
+    have k := k.comp (Primrec.fst (β := Code × Code × Option ℕ × Option ℕ))
+    have n := n.comp (Primrec.fst (β := Code × Code × Option ℕ × Option ℕ))
+    have cf := Primrec.fst.comp (Primrec.snd (α := (List (List (Option ℕ)) × ℕ) × ℕ)
+        (β := Code × Code × Option ℕ × Option ℕ))
+    have cg := (Primrec.fst.comp Primrec.snd).comp
+      (Primrec.snd (α := (List (List (Option ℕ)) × ℕ) × ℕ)
+        (β := Code × Code × Option ℕ × Option ℕ))
+    refine Primrec.option_bind (hlup.comp <| L.pair <| (k.pair cg).pair n) ?_
+    unfold Primrec₂
+    have h :=
+      hlup.comp ((L.comp Primrec.fst).pair <| ((k.pair cf).comp Primrec.fst).pair Primrec.snd)
+    exact h
+  · have L := (Primrec.fst.comp Primrec.fst).comp
+      (Primrec.fst (α := (List (List (Option ℕ)) × ℕ) × ℕ)
+        (β := Code × Code × Option ℕ × Option ℕ))
+    have k := k.comp (Primrec.fst (β := Code × Code × Option ℕ × Option ℕ))
+    have n := n.comp (Primrec.fst (β := Code × Code × Option ℕ × Option ℕ))
+    have cf := Primrec.fst.comp (Primrec.snd (α := (List (List (Option ℕ)) × ℕ) × ℕ)
+        (β := Code × Code × Option ℕ × Option ℕ))
+    have cg := (Primrec.fst.comp Primrec.snd).comp
+      (Primrec.snd (α := (List (List (Option ℕ)) × ℕ) × ℕ)
+        (β := Code × Code × Option ℕ × Option ℕ))
+    have z := Primrec.fst.comp (Primrec.unpair.comp n)
+    refine
+      Primrec.nat_casesOn (Primrec.snd.comp (Primrec.unpair.comp n))
+        (hlup.comp <| L.pair <| (k.pair cf).pair z)
+        (?_ : Primrec _)
+    have L := L.comp (Primrec.fst (β := ℕ))
+    have z := z.comp (Primrec.fst (β := ℕ))
+    have y := Primrec.snd
+      (α := ((List (List (Option ℕ)) × ℕ) × ℕ) × Code × Code × Option ℕ × Option ℕ) (β := ℕ)
+    have h₁ := hlup.comp <| L.pair <| (((k'.pair c).comp Primrec.fst).comp Primrec.fst).pair
+      (Primrec₂.natPair.comp z y)
+    refine Primrec.option_bind h₁ (?_ : Primrec _)
+    have z := z.comp (Primrec.fst (β := ℕ))
+    have y := y.comp (Primrec.fst (β := ℕ))
+    have i := Primrec.snd
+      (α := (((List (List (Option ℕ)) × ℕ) × ℕ) × Code × Code × Option ℕ × Option ℕ) × ℕ)
+      (β := ℕ)
+    have h₂ := hlup.comp ((L.comp Primrec.fst).pair <|
+      ((k.pair cg).comp <| Primrec.fst.comp Primrec.fst).pair <|
+        Primrec₂.natPair.comp z <| Primrec₂.natPair.comp y i)
+    exact h₂
+  · have L := (Primrec.fst.comp Primrec.fst).comp
+      (Primrec.fst (α := (List (List (Option ℕ)) × ℕ) × ℕ)
+        (β := Code × Option ℕ))
+    have k := k.comp (Primrec.fst (β := Code × Option ℕ))
+    have n := n.comp (Primrec.fst (β := Code × Option ℕ))
+    have cf := Primrec.fst.comp (Primrec.snd (α := (List (List (Option ℕ)) × ℕ) × ℕ)
+        (β := Code × Option ℕ))
+    have z := Primrec.fst.comp (Primrec.unpair.comp n)
+    have m := Primrec.snd.comp (Primrec.unpair.comp n)
+    have h₁ := hlup.comp <| L.pair <| (k.pair cf).pair (Primrec₂.natPair.comp z m)
+    refine Primrec.option_bind h₁ (?_ : Primrec _)
+    have m := m.comp (Primrec.fst (β := ℕ))
+    refine Primrec.nat_casesOn Primrec.snd (Primrec.option_some.comp m) ?_
+    unfold Primrec₂
+    exact (hlup.comp ((L.comp Primrec.fst).pair <|
+      ((k'.pair c).comp <| Primrec.fst.comp Primrec.fst).pair
+        (Primrec₂.natPair.comp (z.comp Primrec.fst) (_root_.Primrec.succ.comp m)))).comp
+      Primrec.fst
+-/
 
 -- TODO: What is the right statement of this theorem?
--- private theorem evaln_map (k c n) :
---     ((List.range k)[n]?.bind fun a ↦ evaln k c a) = evaln k c n := by
---   by_cases kn : n < k
---   · simp [List.getElem?_range kn]
---   · rw [List.getElem?_eq_none]
---     · cases e : evaln k c n
---       · rfl
---       exact kn.elim (evaln_bound e)
---     simpa using kn
+/-
+private theorem evaln_map (k c n) :
+    ((List.range k)[n]?.bind fun a ↦ evaln k c a) = evaln k c n := by
+  by_cases kn : n < k
+  · simp [List.getElem?_range kn]
+  · rw [List.getElem?_eq_none]
+    · cases e : evaln k c n
+      · rfl
+      exact kn.elim (evaln_bound e)
+    simpa using kn
+-/
 
 set_option linter.flexible false in -- TODO: revisit this after #13791 is merged
 -- /-- The `Nat.Partrec.Code.evaln` function is primitive recursive. -/
 -- TODO: What is the correct way to state this theorem?
--- theorem primrec_evaln : Primrec fun a : (ℕ × Code) × ℕ => evaln a.1.1 a.1.2 a.2 :=
---   have :
---     Primrec₂ fun (_ : Unit) (n : ℕ) =>
---       let a := ofNat (ℕ × Code) n
---       (List.range a.1).map (evaln a.1 a.2) :=
---     Primrec.nat_strong_rec _ (hG.comp Primrec.snd).to₂ fun _ p => by
---       simp only [G, prod_ofNat_val, ofNat_nat, List.length_map, List.length_range,
---         Nat.pair_unpair, Option.some_inj]
---       refine List.map_congr_left fun n => ?_
---       have : List.range p = List.range (Nat.pair p.unpair.1 (encode (ofNat Code p.unpair.2))) := by
---         simp
---       rw [this]
---       generalize p.unpair.1 = k
---       generalize ofNat Code p.unpair.2 = c
---       intro nk
---       rcases k with - | k'
---       · simp [evaln]
---       let k := k' + 1
---       simp only
---       simp only [List.mem_range, Nat.lt_succ_iff] at nk
---       have hg :
---         ∀ {k' c' n},
---           Nat.pair k' (encode c') < Nat.pair k (encode c) →
---             lup ((List.range (Nat.pair k (encode c))).map fun n =>
---               (List.range n.unpair.1).map (evaln n.unpair.1 (ofNat Code n.unpair.2))) (k', c') n =
---             evaln k' c' n := by
---         intro k₁ c₁ n₁ hl
---         simp [lup, List.getElem?_range hl, evaln_map, Bind.bind, Option.bind_map]
---       obtain - | - | - | - | ⟨cf, cg⟩ | ⟨cf, cg⟩ | ⟨cf, cg⟩ | cf := c <;>
---         simp [evaln, nk, Bind.bind, Functor.map, Seq.seq, pure]
---       · obtain ⟨lf, lg⟩ := encode_lt_pair cf cg
---         rw [hg (Nat.pair_lt_pair_right _ lf), hg (Nat.pair_lt_pair_right _ lg)]
---         cases evaln k cf n
---         · rfl
---         cases evaln k cg n <;> rfl
---       · obtain ⟨lf, lg⟩ := encode_lt_comp cf cg
---         rw [hg (Nat.pair_lt_pair_right _ lg)]
---         cases evaln k cg n
---         · rfl
---         simp [k, hg (Nat.pair_lt_pair_right _ lf)]
---       · obtain ⟨lf, lg⟩ := encode_lt_prec cf cg
---         rw [hg (Nat.pair_lt_pair_right _ lf)]
---         cases n.unpair.2
---         · rfl
---         simp only
---         rw [hg (Nat.pair_lt_pair_left _ k'.lt_succ_self)]
---         cases evaln k' _ _
---         · rfl
---         simp [k, hg (Nat.pair_lt_pair_right _ lg)]
---       · have lf := encode_lt_rfind' cf
---         rw [hg (Nat.pair_lt_pair_right _ lf)]
---         rcases evaln k cf n with - | x
---         · rfl
---         simp only [Option.bind_some]
---         cases x <;> simp
---         rw [hg (Nat.pair_lt_pair_left _ k'.lt_succ_self)]
---   (Primrec.option_bind
---     (Primrec.list_getElem?.comp (this.comp (_root_.Primrec.const ())
---       (Primrec.encode_iff.2 Primrec.fst)) Primrec.snd) Primrec.snd.to₂).of_eq
---     fun ⟨⟨k, c⟩, n⟩ => by simp [evaln_map, Option.bind_map]
+/-
+theorem primrec_evaln : Primrec fun a : (ℕ × Code) × ℕ => evaln a.1.1 a.1.2 a.2 :=
+  have :
+    Primrec₂ fun (_ : Unit) (n : ℕ) =>
+      let a := ofNat (ℕ × Code) n
+      (List.range a.1).map (evaln a.1 a.2) :=
+    Primrec.nat_strong_rec _ (hG.comp Primrec.snd).to₂ fun _ p => by
+      simp only [G, prod_ofNat_val, ofNat_nat, List.length_map, List.length_range,
+        Nat.pair_unpair, Option.some_inj]
+      refine List.map_congr_left fun n => ?_
+      have : List.range p = List.range (Nat.pair p.unpair.1 (encode (ofNat Code p.unpair.2))) := by
+        simp
+      rw [this]
+      generalize p.unpair.1 = k
+      generalize ofNat Code p.unpair.2 = c
+      intro nk
+      rcases k with - | k'
+      · simp [evaln]
+      let k := k' + 1
+      simp only
+      simp only [List.mem_range, Nat.lt_succ_iff] at nk
+      have hg :
+        ∀ {k' c' n},
+          Nat.pair k' (encode c') < Nat.pair k (encode c) →
+            lup ((List.range (Nat.pair k (encode c))).map fun n =>
+              (List.range n.unpair.1).map (evaln n.unpair.1 (ofNat Code n.unpair.2))) (k', c') n =
+            evaln k' c' n := by
+        intro k₁ c₁ n₁ hl
+        simp [lup, List.getElem?_range hl, evaln_map, Bind.bind, Option.bind_map]
+      obtain - | - | - | - | ⟨cf, cg⟩ | ⟨cf, cg⟩ | ⟨cf, cg⟩ | cf := c <;>
+        simp [evaln, nk, Bind.bind, Functor.map, Seq.seq, pure]
+      · obtain ⟨lf, lg⟩ := encode_lt_pair cf cg
+        rw [hg (Nat.pair_lt_pair_right _ lf), hg (Nat.pair_lt_pair_right _ lg)]
+        cases evaln k cf n
+        · rfl
+        cases evaln k cg n <;> rfl
+      · obtain ⟨lf, lg⟩ := encode_lt_comp cf cg
+        rw [hg (Nat.pair_lt_pair_right _ lg)]
+        cases evaln k cg n
+        · rfl
+        simp [k, hg (Nat.pair_lt_pair_right _ lf)]
+      · obtain ⟨lf, lg⟩ := encode_lt_prec cf cg
+        rw [hg (Nat.pair_lt_pair_right _ lf)]
+        cases n.unpair.2
+        · rfl
+        simp only
+        rw [hg (Nat.pair_lt_pair_left _ k'.lt_succ_self)]
+        cases evaln k' _ _
+        · rfl
+        simp [k, hg (Nat.pair_lt_pair_right _ lg)]
+      · have lf := encode_lt_rfind' cf
+        rw [hg (Nat.pair_lt_pair_right _ lf)]
+        rcases evaln k cf n with - | x
+        · rfl
+        simp only [Option.bind_some]
+        cases x <;> simp
+        rw [hg (Nat.pair_lt_pair_left _ k'.lt_succ_self)]
+  (Primrec.option_bind
+    (Primrec.list_getElem?.comp (this.comp (_root_.Primrec.const ())
+      (Primrec.encode_iff.2 Primrec.fst)) Primrec.snd) Primrec.snd.to₂).of_eq
+    fun ⟨⟨k, c⟩, n⟩ => by simp [evaln_map, Option.bind_map]
+-/
 
 end
 
@@ -1015,47 +1027,55 @@ section
 open Partrec Computable
 
 -- TODO: do we need to update this?
--- theorem eval_eq_rfindOpt (c n) : eval c n = Nat.rfindOpt fun k => evaln k c n :=
---   Part.ext fun x => by
---     refine evaln_complete.trans (Nat.rfindOpt_mono ?_).symm
---     intro a m n hl; apply evaln_mono hl
+/-
+theorem eval_eq_rfindOpt (c n) : eval c n = Nat.rfindOpt fun k => evaln k c n :=
+  Part.ext fun x => by
+    refine evaln_complete.trans (Nat.rfindOpt_mono ?_).symm
+    intro a m n hl; apply evaln_mono hl
+-/
 
 -- TODO: do we need to update this?
--- theorem eval_part : Partrec₂ eval :=
---   (Partrec.rfindOpt
---     (primrec_evaln.to_comp.comp
---       ((Computable.snd.pair (fst.comp fst)).pair (snd.comp fst))).to₂).of_eq
---     fun a => by simp [eval_eq_rfindOpt]
+/-
+theorem eval_part : Partrec₂ eval :=
+  (Partrec.rfindOpt
+    (primrec_evaln.to_comp.comp
+      ((Computable.snd.pair (fst.comp fst)).pair (snd.comp fst))).to₂).of_eq
+    fun a => by simp [eval_eq_rfindOpt]
+-/
 
 -- /-- **Roger's fixed-point theorem**: any total, computable `f` has a fixed point.
 -- That is, under the interpretation given by `Nat.Partrec.Code.eval`, there is a code `c`
 -- such that `c` and `f c` have the same evaluation.
 -- -/
 -- TODO: What is the correct relativization of this theorem?
--- theorem fixed_point {f : OCode → OCode} (hf : Computable f) : ∃ c : OCode, eval (f c) = eval c :=
---   let g (x y : ℕ) : Part ℕ := eval (ofNat Code x) x >>= fun b => eval (ofNat Code b) y
---   have : Partrec₂ g :=
---     (eval_part.comp ((Computable.ofNat _).comp fst) fst).bind
---       (eval_part.comp ((Computable.ofNat _).comp snd) (snd.comp fst)).to₂
---   let ⟨cg, eg⟩ := exists_code.1 this
---   have eg' : ∀ a n, eval cg (Nat.pair a n) = Part.map encode (g a n) := by simp [eg]
---   let F (x : ℕ) : Code := f (curry cg x)
---   have : Computable F :=
---     hf.comp (primrec₂_curry.comp (_root_.Primrec.const cg) _root_.Primrec.id).to_comp
---   let ⟨cF, eF⟩ := exists_code.1 this
---   have eF' : eval cF (encode cF) = Part.some (encode (F (encode cF))) := by simp [eF]
---   ⟨curry cg (encode cF),
---     funext fun n =>
---       show eval (f (curry cg (encode cF))) n = eval (curry cg (encode cF)) n by
---         simp [F, g, eg', eF', Part.map_id']⟩
+/-
+theorem fixed_point {f : Code → Code} (hf : Computable f) : ∃ c : Code, eval (f c) = eval c :=
+  let g (x y : ℕ) : Part ℕ := eval (ofNat Code x) x >>= fun b => eval (ofNat Code b) y
+  have : Partrec₂ g :=
+    (eval_part.comp ((Computable.ofNat _).comp fst) fst).bind
+      (eval_part.comp ((Computable.ofNat _).comp snd) (snd.comp fst)).to₂
+  let ⟨cg, eg⟩ := exists_code.1 this
+  have eg' : ∀ a n, eval cg (Nat.pair a n) = Part.map encode (g a n) := by simp [eg]
+  let F (x : ℕ) : Code := f (curry cg x)
+  have : Computable F :=
+    hf.comp (primrec₂_curry.comp (_root_.Primrec.const cg) _root_.Primrec.id).to_comp
+  let ⟨cF, eF⟩ := exists_code.1 this
+  have eF' : eval cF (encode cF) = Part.some (encode (F (encode cF))) := by simp [eF]
+  ⟨curry cg (encode cF),
+    funext fun n =>
+      show eval (f (curry cg (encode cF))) n = eval (curry cg (encode cF)) n by
+        simp [F, g, eg', eF', Part.map_id']⟩
+-/
 
 -- /-- **Kleene's second recursion theorem** -/
 -- TODO: What is the correct relativization of this theorem?
--- theorem fixed_point₂ {f : Code → ℕ →. ℕ} (hf : Partrec₂ f) : ∃ c : Code, eval c = f c :=
---   let ⟨cf, ef⟩ := exists_code.1 hf
---   (fixed_point (primrec₂_curry.comp (_root_.Primrec.const cf) Primrec.encode).to_comp).imp
---     fun c e => funext fun n => by simp [e.symm, ef, Part.map_id']
+/-
+theorem fixed_point₂ {f : Code → ℕ →. ℕ} (hf : Partrec₂ f) : ∃ c : Code, eval c = f c :=
+  let ⟨cf, ef⟩ := exists_code.1 hf
+  (fixed_point (primrec₂_curry.comp (_root_.Primrec.const cf) Primrec.encode).to_comp).imp
+    fun c e => funext fun n => by simp [e.symm, ef, Part.map_id']
+-/
 
 end
 
-end RecursiveIn.OCode
+end RecursiveIn.Code
